Hoare/TerminationTriple.thy
@@ -1,75 +1,325 @@
 theory TerminationTriple
-imports "EvmFacts" "./Hoare"  "HoareTripleForInstructions"
+imports "EvmFacts" "./Hoare"
+  "HoareTripleForInstructions"
 
 begin
-
-
-
-(*
-lemma gas_decreases_in_triples :
- "vctx_gas v2 \<ge> vctx_gas v1 \<Longrightarrow>
-  (all_but_gas ** gas_pred g) (contexts_as_set v1 c) \<Longrightarrow>
-  (all_but_gas ** gas_pred g2) (contexts_as_set v2 c)"
-apply(auto simp add:rw sep_def gas_smaller_def
-  not_continuing_def all_but_gas_def
-         failing_def some_gas_def code_def
- gas_pred_def context_rw)
-*)
 
 definition all_context :: "state_element set_pred" where
 "all_context s = (\<exists>c v.  s = contexts_as_set v c)"
 
-lemma gas_decreases_in_triples :
+lemma context_maximal :
  "(rest ** all_context) (contexts_as_set v1 c) \<Longrightarrow>
   rest {}"
+  by (smt Un_upper2 all_context_def inf_sup_absorb maximality sep_def)
 
-lemma gas_decreases_in_triples :
+lemma all_context_rest :
  "(rest ** all_context) (contexts_as_set v1 c) \<Longrightarrow>
   (rest ** all_context) (contexts_as_set v2 c)"
+  by (metis all_context_def context_maximal inf_bot_right sep_def set_pred.commute sup_bot.right_neutral)
 
+(*
 lemma gas_decreases_in_triples :
  "vctx_gas v2 \<ge> vctx_gas v1 \<Longrightarrow>
   (all ** gas_pred g) (contexts_as_set v1 c) \<Longrightarrow>
   (all ** gas_smaller g) (contexts_as_set v2 c)"
+*)
 
-lemma foo_helper [simp] :
-"(rest **
-        all ** continuing ** code {} ** gas_pred g)
-        (insert (ContinuingElm True)
-          (contexts_as_set x1 co_ctx)) =
-  (rest ** all ** code {} ** gas_pred g)
-    (contexts_as_set x1 co_ctx)"
-apply (auto simp add:context_rw)
+definition all_with_gas :: "int \<Rightarrow> state_element set_pred" where
+"all_with_gas g s = (\<exists>c v.  s = contexts_as_set v c \<and>
+   vctx_gas v = g \<and> vctx_memory_usage v \<ge> 0)"
+
+definition all_with_less_gas :: "int \<Rightarrow> state_element set_pred" where
+"all_with_less_gas g s = (\<exists>c v.  s = contexts_as_set v c \<and>
+   vctx_gas v < g \<and> vctx_memory_usage v \<ge> 0)"
+
+definition all_perhaps_less_gas :: "int \<Rightarrow> state_element set_pred" where
+"all_perhaps_less_gas g s = (\<exists>c v.  s = contexts_as_set v c \<and>
+   vctx_gas v \<le> g \<and> vctx_memory_usage v \<ge> 0)"
+
+
+lemma some_gas_in_context :
+"(rest ** all_with_gas g) s \<Longrightarrow>
+ (rest ** all_perhaps_less_gas g) s"
+apply(auto simp add:rw sep_def  not_continuing_def
+   all_context_def
+   all_with_gas_def
+   all_perhaps_less_gas_def
+         failing_def some_gas_def code_def)
+done
+
+lemma case_1 :
+assumes a :
+ "(rest ** all_with_gas g) (contexts_as_set x1 co_ctx)"
+shows  "(rest ** not_continuing ** all_perhaps_less_gas g ** failing)
+           (insert (ContinuingElm False)
+             (insert
+               (ContractActionElm (ContractFail lst))
+               (contexts_as_set x1 co_ctx)))"
+proof -
+  let ?set =  "contexts_as_set x1 co_ctx"
+  let ?base =  "rest ** all_perhaps_less_gas g"
+from a have "?base ?set" using some_gas_in_context by force
+then have "(?base ** not_continuing) (insert (ContinuingElm False) ?set)"
+  using context_cont1 not_cont_insert by presburger
+then have "(?base ** not_continuing)
+   (insert (ContinuingElm False) ?set-{ContractActionElm (ContractFail lst)})"
+  by (metis (full_types) Diff_empty Diff_insert2 context_cont context_cont1 contexts_as_set_def insert_minus state_element.distinct(685))
+then show ?thesis
+  by (metis failing_insert insert_commute sep_three set_pred.commute) 
+qed
+
+lemma funext : "(\<forall>x. f x = g x) \<Longrightarrow> f = g"
+by auto
+
+lemma code_emp [simp] : "code {} = emp"
+apply (rule funext)
+apply (simp add:emp_def code_def)
+done
+
+lemma all_with_gas_max :
+   "(rest ** all_with_gas g) (contexts_as_set v1 co_ctx) \<Longrightarrow>
+    rest {}"
+  by (smt all_with_gas_def inf_sup_absorb maximality sep_def sup.cobounded2)
+
+lemma all_with_gas_memu :
+   "(rest ** all_with_gas g) (contexts_as_set v1 co_ctx) \<Longrightarrow>
+    vctx_memory_usage v1 \<ge> 0"
+  by (smt Un_upper2 all_with_gas_def get_condition1 sep_def)
+
+lemma all_with_gas_gas :
+   "(rest ** all_with_gas g) (contexts_as_set v1 co_ctx) \<Longrightarrow>
+    vctx_gas v1 = g"
+  by (smt Un_upper2 all_with_gas_def get_condition1 sep_def)
+
+lemma construct_less_gas :
+"vctx_memory_usage v2 \<ge> 0 \<Longrightarrow> vctx_gas v2 < g \<Longrightarrow>
+ rest {} \<Longrightarrow>
+ (rest ** all_with_less_gas g) (contexts_as_set v2 co_ctx)"
+  by (metis all_with_less_gas_def emp_def imp_sepL sep_emp set_pred.commute)
+
+lemma construct_perhaps_gas :
+"vctx_memory_usage v2 \<ge> 0 \<Longrightarrow> vctx_gas v2 \<le> g \<Longrightarrow>
+ rest {} \<Longrightarrow>
+ (rest ** all_perhaps_less_gas g) (contexts_as_set v2 co_ctx)"
+  by (metis all_perhaps_less_gas_def emp_def imp_sepL sep_emp set_pred.commute)
+
+lemma normal_case : assumes
+ a:"(rest ** all_with_gas g) (contexts_as_set v1 co_ctx)" and
+ b:"instruction_sem v1 co_ctx inst = InstructionContinue v2"
+ shows  "(rest ** all_with_less_gas g) (contexts_as_set v2 co_ctx)"
+proof -
+  from a have "vctx_memory_usage v1 \<ge> 0 \<and> vctx_gas v1 = g"
+    using all_with_gas_gas all_with_gas_memu by auto
+  then have "vctx_memory_usage v2 \<ge> 0 \<and> vctx_gas v2 < g"
+   using b continue_decr_gas memu_good by fastforce
+  then show ?thesis using construct_less_gas all_with_gas_max a by fastforce
+qed
+
+lemma add_action :
+"rest (insert (ContinuingElm False)
+     (contexts_as_set v2 co_ctx)) \<Longrightarrow>
+ pred act \<Longrightarrow>
+ (action pred ** rest)
+     (instruction_result_as_set co_ctx
+       (InstructionToEnvironment act v2 x33))"
+apply (simp add: instruction_result_as_set_def
+              action_def sep_def action_not_context)
+apply force
+done
+
+lemma call_case : assumes
+ a:"(rest ** all_with_gas g) (contexts_as_set v1 co_ctx)" and
+ b:"instruction_sem v1 co_ctx inst =
+    InstructionToEnvironment (ContractCall x1) v2 x33"
+ shows "(calling ** not_continuing **
+           rest ** all_with_less_gas g)
+           (instruction_result_as_set co_ctx
+             (InstructionToEnvironment
+               (ContractCall x1) v2 x33))"
+proof -
+  from a have "vctx_memory_usage v1 \<ge> 0 \<and> vctx_gas v1 = g"
+    using all_with_gas_gas all_with_gas_memu by auto
+  then have "vctx_memory_usage v2 \<ge> 0 \<and> vctx_gas v2 < g"
+   using b call_decr_gas memu_good_env by fastforce
+  then have "(rest ** all_with_less_gas g) (contexts_as_set v2 co_ctx)"
+   using construct_less_gas all_with_gas_max a by fastforce
+  then have "(not_continuing ** rest ** all_with_less_gas g)
+    (insert (ContinuingElm False) (contexts_as_set v2 co_ctx))"
+    by (simp add: not_continuing_sep)
+  then show ?thesis  by (smt add_action calling_def)
+qed
+
+lemma delegatecall_case : assumes
+ a:"(rest ** all_with_gas g) (contexts_as_set v1 co_ctx)" and
+ b:"instruction_sem v1 co_ctx inst =
+    InstructionToEnvironment (ContractDelegateCall x1) v2 x33"
+ shows "(delegating ** not_continuing **
+           rest ** all_with_less_gas g)
+           (instruction_result_as_set co_ctx
+             (InstructionToEnvironment
+               (ContractDelegateCall x1) v2 x33))"
+proof -
+  from a have "vctx_memory_usage v1 \<ge> 0 \<and> vctx_gas v1 = g"
+    using all_with_gas_gas all_with_gas_memu by auto
+  then have "vctx_memory_usage v2 \<ge> 0 \<and> vctx_gas v2 < g"
+   using b delegatecall_decr_gas memu_good_env by fastforce
+  then have "(rest ** all_with_less_gas g) (contexts_as_set v2 co_ctx)"
+   using construct_less_gas all_with_gas_max a by fastforce
+  then have "(not_continuing ** rest ** all_with_less_gas g)
+    (insert (ContinuingElm False) (contexts_as_set v2 co_ctx))"
+    by (simp add: not_continuing_sep)
+  then show ?thesis by (smt add_action delegating_def)
+qed
+
+lemma create_case : assumes
+ a:"(rest ** all_with_gas g) (contexts_as_set v1 co_ctx)" and
+ b:"instruction_sem v1 co_ctx inst =
+    InstructionToEnvironment (ContractCreate x1) v2 x33"
+ shows "(creating ** not_continuing **
+           rest ** all_with_less_gas g)
+           (instruction_result_as_set co_ctx
+             (InstructionToEnvironment
+               (ContractCreate x1) v2 x33))"
+proof -
+  from a have "vctx_memory_usage v1 \<ge> 0 \<and> vctx_gas v1 = g"
+    using all_with_gas_gas all_with_gas_memu by auto
+  then have "vctx_memory_usage v2 \<ge> 0 \<and> vctx_gas v2 < g"
+   using b create_decr_gas memu_good_env by fastforce
+  then have "(rest ** all_with_less_gas g) (contexts_as_set v2 co_ctx)"
+   using construct_less_gas all_with_gas_max a by fastforce
+  then have "(not_continuing ** rest ** all_with_less_gas g)
+    (insert (ContinuingElm False) (contexts_as_set v2 co_ctx))"
+    by (simp add: not_continuing_sep)
+  then show ?thesis by (smt add_action creating_def)
+qed
+
+lemma fail_case : assumes
+ a:"(rest ** all_with_gas g) (contexts_as_set v1 co_ctx)" and
+ b:"instruction_sem v1 co_ctx inst =
+    InstructionToEnvironment (ContractFail x1) v2 x33"
+ shows "(failing ** not_continuing **
+           rest ** all_perhaps_less_gas g)
+           (instruction_result_as_set co_ctx
+             (InstructionToEnvironment
+               (ContractFail x1) v2 x33))"
+proof -
+  from a have "vctx_memory_usage v1 \<ge> 0 \<and> vctx_gas v1 = g"
+    using all_with_gas_gas all_with_gas_memu by auto
+  then have "vctx_memory_usage v2 \<ge> 0 \<and> vctx_gas v2 \<le> g"
+   using b memu_good_env env_meter_gas meter_gas_ge_0 by fastforce 
+  then have "(rest ** all_perhaps_less_gas g) (contexts_as_set v2 co_ctx)"
+   using construct_perhaps_gas all_with_gas_max a by fastforce
+  then have "(not_continuing ** rest ** all_perhaps_less_gas g)
+    (insert (ContinuingElm False) (contexts_as_set v2 co_ctx))"
+    by (simp add: not_continuing_sep)
+  then show ?thesis by (smt add_action failing_def)
+qed
+
+lemma suicide_case : assumes
+ a:"(rest ** all_with_gas g) (contexts_as_set v1 co_ctx)" and
+ b:"instruction_sem v1 co_ctx inst =
+    InstructionToEnvironment (ContractSuicide x1) v2 x33"
+ shows "(destructing ** not_continuing **
+           rest ** all_perhaps_less_gas g)
+           (instruction_result_as_set co_ctx
+             (InstructionToEnvironment
+               (ContractSuicide x1) v2 x33))"
+proof -
+  from a have "vctx_memory_usage v1 \<ge> 0 \<and> vctx_gas v1 = g"
+    using all_with_gas_gas all_with_gas_memu by auto
+  then have "vctx_memory_usage v2 \<ge> 0 \<and> vctx_gas v2 \<le> g"
+   using b memu_good_env env_meter_gas meter_gas_ge_0 by fastforce 
+  then have "(rest ** all_perhaps_less_gas g) (contexts_as_set v2 co_ctx)"
+   using construct_perhaps_gas all_with_gas_max a by fastforce
+  then have "(not_continuing ** rest ** all_perhaps_less_gas g)
+    (insert (ContinuingElm False) (contexts_as_set v2 co_ctx))"
+    by (simp add: not_continuing_sep)
+  then show ?thesis
+    using add_action
+      [of "not_continuing ** rest ** all_perhaps_less_gas g" v2 co_ctx
+        "\<lambda>y. \<exists>x. ContractSuicide x = y" "ContractSuicide x1" x33]
+    by (simp add: destructing_def)
+    
+qed
+
+lemma return_case : assumes
+ a:"(rest ** all_with_gas g) (contexts_as_set v1 co_ctx)" and
+ b:"instruction_sem v1 co_ctx inst =
+    InstructionToEnvironment (ContractReturn x1) v2 x33"
+ shows "(returning ** not_continuing **
+           rest ** all_perhaps_less_gas g)
+           (instruction_result_as_set co_ctx
+             (InstructionToEnvironment
+               (ContractReturn x1) v2 x33))"
+proof -
+  from a have "vctx_memory_usage v1 \<ge> 0 \<and> vctx_gas v1 = g"
+    using all_with_gas_gas all_with_gas_memu by auto
+  then have "vctx_memory_usage v2 \<ge> 0 \<and> vctx_gas v2 \<le> g"
+   using b memu_good_env env_meter_gas meter_gas_ge_0 by fastforce 
+  then have "(rest ** all_perhaps_less_gas g) (contexts_as_set v2 co_ctx)"
+   using construct_perhaps_gas all_with_gas_max a by fastforce
+  then have "(not_continuing ** rest ** all_perhaps_less_gas g)
+    (insert (ContinuingElm False) (contexts_as_set v2 co_ctx))"
+    by (simp add: not_continuing_sep)
+  then show ?thesis by (smt add_action returning_def)
+qed
+
+lemma simple :
+"instruction_result_as_set co_ctx
+          (InstructionContinue v1) -
+         {ContinuingElm True} = contexts_as_set v1 co_ctx"
+apply (simp add:instruction_result_as_set_def)
 done
 
 lemma using_gas_triple :
-   "triple {} (gas_pred g ** continuing ** all) {}
-    (gas_smaller g ** continuing ** all
-    ## gas_smaller g ** all ** not_continuing **
-      (delegating ## calling ## creating ## destructing)
-    ## all ** some_gas ** not_continuing **
-       (failing ## returning))"
+   "triple {} (all_with_gas g ** continuing) {}
+    (all_with_less_gas g ** continuing 
+    ## all_with_less_gas g ** not_continuing **
+      (delegating ## calling ## creating)
+    ## all_perhaps_less_gas g ** not_continuing **
+       (failing ## returning  ## destructing))"
 apply(auto simp add: triple_def)
  apply(rule_tac x = 1 in exI)
  apply(case_tac presult; auto)
-apply (simp add:sep_add_def instruction_result_as_set_def
+apply (simp add:sep_add_def 
   program_sem.simps next_state_def)
 apply (case_tac "vctx_next_instruction x1 co_ctx")
-apply auto
+apply (auto simp add:case_1 meter_gas_check)
+apply (simp add: instruction_result_as_set_def)
 using case_1 apply force
 defer
+defer
+apply (simp add: instruction_result_as_set_def)
 using case_1 apply force
 using meter_gas_check apply force
+using meter_gas_check apply force
+apply (simp add: instruction_result_as_set_def)
 using case_1 apply force
-  apply (metis (mono_tags) sep_continuing_sep sep_lc singleton_iff state_element.inject(21))
-  apply (metis instruction_result_as_set_def sep_continuing_sep set_pred.left_commute to_environment_not_continuing)
-apply (case_tac "instruction_sem x1 co_ctx a"; auto)
-defer
-using no_annotation_inst apply force
-apply (case_tac x31; auto)
+subgoal for co_ctx rest v1 inst
+apply (case_tac "instruction_sem v1 co_ctx inst"; auto)
+apply (simp add: instruction_result_as_set_def)
+using no_annotation_inst apply simp
+apply (case_tac x31; auto simp:simple)
+using call_case apply force
+using delegatecall_case apply force
+using create_case apply force
+using fail_case apply force
+using suicide_case apply force
+using return_case apply force
+done
+subgoal for co_ctx rest v1 inst
+apply (case_tac "instruction_sem v1 co_ctx inst"; auto)
+apply (simp add: instruction_result_as_set_def)
+using normal_case apply simp
+using no_annotation_inst apply simp
+apply (case_tac x31; auto simp:simple)
+using call_case apply force
+using delegatecall_case apply force
+using create_case apply force
+using fail_case apply force
+using suicide_case apply force
+using return_case apply force
+done
+done
 
-
-(*
- auto simp add: instruction_result_as_set_def sep_def sep_add_def)
-*)
 end
